Added proof for new IntegerEqualsNode optimisation. Fixed a failing proof.

Optimizations/Canonicalizations/ConditionalPhase.thy
@@ -31,8 +31,9 @@ lemma negation_preserve_eval_intval:
   by (metis assms eval_bits_1_64 intval_logic_negation.elims negation_preserve_eval unfold_unary)
 
 optimization NegateConditionFlipBranches: "((!e) ? x : y) \<longmapsto> (e ? y : x)"
-  by (smt (verit, ccfv_SIG) le_expr_def ConditionalExpr ConditionalExprE Value.distinct(1) evalDet 
-      negates negation_preserve_eval negation_preserve_eval_intval)
+  apply simp
+  by (smt (z3) le_expr_def ConditionalExpr ConditionalExprE Value.distinct(1) evalDet negates
+      negation_preserve_eval negation_preserve_eval_intval)
 
 optimization DefaultTrueBranch: "(true ? x : y) \<longmapsto> x" .
 
@@ -62,9 +63,153 @@ lemma val_optimise_integer_test:
 optimization ConditionalEliminateKnownLess: "((x < y) ? x : y) \<longmapsto> x 
                                  when (stamp_under (stamp_expr x) (stamp_expr y)
                                       \<and> wf_stamp x \<and> wf_stamp y)"
-    using stamp_under_defn by fastforce
+  using stamp_under_defn by fastforce
+
+lemma ExpIntBecomesIntVal:
+  assumes "stamp_expr x = IntegerStamp b xl xh"
+  assumes "wf_stamp x"
+  assumes "valid_value v (IntegerStamp b xl xh)"
+  assumes "[m,p] \<turnstile> x \<mapsto> v"
+  shows "\<exists>xv. v = IntVal b xv"
+  using assms by (simp add: IRTreeEvalThms.valid_value_elims(3))
 
 (* Optimisations *)
+
+lemma intval_self_is_true:
+  assumes "yv \<noteq> UndefVal"
+  assumes "yv = IntVal b yvv"
+  shows "intval_equals yv yv = IntVal 32 1"
+  using assms by (cases yv; auto)
+
+lemma intval_commute:
+  assumes "intval_equals yv xv \<noteq> UndefVal"
+  assumes "intval_equals xv yv \<noteq> UndefVal"
+  shows "intval_equals yv xv = intval_equals xv yv"
+  using assms apply (cases yv; cases xv; auto) by (smt (verit, best))
+
+definition isBoolean :: "IRExpr \<Rightarrow> bool" where
+  "isBoolean e = (\<forall>m p cond. (([m,p] \<turnstile> e \<mapsto> cond) \<longrightarrow> (cond \<in> {IntVal 32 0, IntVal 32 1})))"
+
+optimization ConditionalIntegerEquals_1: "exp[BinaryExpr BinIntegerEquals (c ? x : y) (x)] \<longmapsto> c
+                                          when stamp_expr x = IntegerStamp b xl xh \<and> wf_stamp x \<and>
+                                               stamp_expr y = IntegerStamp b yl yh \<and> wf_stamp y \<and>
+                                               (alwaysDistinct (stamp_expr x) (stamp_expr y)) \<and>
+                                               isBoolean c"
+  apply (metis Canonicalization.cond_size add_lessD1 size_binary_lhs) apply auto
+  subgoal premises p for m p cExpr xv cond
+  proof -
+    obtain cond where cond: "[m,p] \<turnstile> c \<mapsto> cond"
+      using p by blast
+    have cRange: "cond = IntVal 32 0 \<or> cond = IntVal 32 1"
+      using p cond isBoolean_def by blast
+    then obtain yv where yVal: "[m,p] \<turnstile> y \<mapsto> yv"
+      using p(15) by auto
+    obtain xvv where xvv: "xv = IntVal b xvv"
+       by (metis p(1,2,7) valid_int wf_stamp_def)
+    obtain yvv where yvv: "yv = IntVal b yvv"
+      using ExpIntBecomesIntVal p(3) p(4) wf_stamp_def
+      using yVal by force
+    have yxDiff: "xv \<noteq> yv"
+       by (smt (verit, ccfv_threshold) yVal xvv wf_stamp_def valid_int_signed_range p)
+    have eqEvalFalse: "intval_equals yv xv = (IntVal 32 0)"
+      unfolding xvv yvv apply auto by (metis (mono_tags) bool_to_val.simps(2) yxDiff yvv xvv)
+    then show ?thesis
+      by (smt (verit) xvv intval_self_is_true yVal p(7,9,11,12) cRange cond val_to_bool.simps(1)
+          evalDet)
+  qed
+  done
+
+(* Helpers *)
+lemma negation_preserve_eval0:
+  assumes "[m, p] \<turnstile> exp[e] \<mapsto> v"
+  assumes "isBoolean e"
+  shows "\<exists>v'. ([m, p] \<turnstile> exp[!e] \<mapsto> v')"
+  using assms
+proof -
+  obtain b vv where vIntVal: "v = IntVal b vv"
+    using isBoolean_def assms by blast
+  then have negationDefined: "intval_logic_negation v \<noteq> UndefVal"
+    by simp
+  show ?thesis
+    using assms(1) negationDefined by fastforce
+qed
+
+lemma negation_preserve_eval2:
+  assumes "([m, p] \<turnstile> exp[e] \<mapsto> v)"
+  assumes "(isBoolean e)"
+  shows "\<exists>v'. ([m, p] \<turnstile> exp[!e] \<mapsto> v') \<and> v = val[!v']"
+  using assms
+proof -
+  obtain notEval where notEval: "([m, p] \<turnstile> exp[!e] \<mapsto> notEval)"
+    by (metis assms negation_preserve_eval0)
+  then have logicNegateEquiv: "notEval = intval_logic_negation v"
+    using evalDet  assms(1) unary_eval.simps(4) by blast
+  then have vRange: "v = IntVal 32 0 \<or> v = IntVal 32 1"
+    using assms by (auto simp add: isBoolean_def)
+  have evaluateNot: "v = intval_logic_negation notEval"
+    by (metis IntVal0 IntVal1 intval_logic_negation.simps(1) logicNegateEquiv logic_negate_def
+        vRange)
+  then show ?thesis
+    using notEval by auto
+qed
+
+optimization ConditionalIntegerEquals_2: "exp[BinaryExpr BinIntegerEquals (c ? x : y) (y)] \<longmapsto> (!c)
+                                          when stamp_expr x = IntegerStamp b xl xh \<and> wf_stamp x \<and>
+                                               stamp_expr y = IntegerStamp b yl yh \<and> wf_stamp y \<and>
+                                               (alwaysDistinct (stamp_expr x) (stamp_expr y)) \<and>
+                                               isBoolean c"
+  apply (smt (verit) not_add_less1 max_less_iff_conj max.absorb3 linorder_less_linear add_2_eq_Suc'
+         add_less_cancel_right size_binary_lhs add_lessD1 Canonicalization.cond_size)
+  apply auto
+  subgoal premises p for m p cExpr yv cond trE faE
+  proof -
+    obtain cond where cond: "[m,p] \<turnstile> c \<mapsto> cond"
+      using p by blast
+    then have condNotUndef: "cond \<noteq> UndefVal"
+      by (simp add: evaltree_not_undef)
+    then obtain notCond where notCond: "[m,p] \<turnstile> exp[!c] \<mapsto> notCond"
+      by (meson p(6) negation_preserve_eval2 cond)
+    have cRange: "cond = IntVal 32 0 \<or> cond = IntVal 32 1"
+      using p cond by (simp add: isBoolean_def)
+    then have cNotRange:  "notCond = IntVal 32 0 \<or> notCond = IntVal 32 1"
+      by (metis (no_types, lifting) IntVal0 IntVal1 cond evalDet intval_logic_negation.simps(1)
+          logic_negate_def negation_preserve_eval notCond)
+    then obtain xv where xv: "[m,p] \<turnstile> x \<mapsto> xv"
+      using p by auto
+    then have trueCond: "(notCond = IntVal 32 1) \<Longrightarrow> [m,p] \<turnstile> (ConditionalExpr c x y) \<mapsto> yv"
+      by (smt (verit, ccfv_SIG) cRange evalDet negates negation_preserve_eval notCond p(7) cond
+          zero_less_numeral val_to_bool.simps(1) evaltree_not_undef ConditionalExpr)
+    obtain xvv where xvv: "xv = IntVal b xvv"
+      by (metis p(1,2) valid_int wf_stamp_def xv)
+     have falseCond: "(notCond = IntVal 32 0) \<Longrightarrow> [m,p] \<turnstile> (ConditionalExpr c x y) \<mapsto> xv"
+      by (smt (verit, ccfv_SIG) evalDet eval_bits_1_64 negates negation_preserve_eval2 notCond xv p
+          val_to_bool.simps(1) evaltree_not_undef ConditionalExpr)
+    obtain yvv where yvv: "yv = IntVal b yvv"
+      by (metis p(3,4,7) wf_stamp_def ExpIntBecomesIntVal)
+    have yxDiff: "xv \<noteq> yv"
+      by (smt (verit, ccfv_threshold) xv yvv wf_stamp_def valid_int_signed_range p)
+    then have trueEvalCond: "(cond = IntVal 32 0) \<Longrightarrow>
+                         [m,p] \<turnstile> exp[BinaryExpr BinIntegerEquals (c ? x : y) (y)]
+                               \<mapsto> intval_equals yv yv"
+      by (smt (verit, best) cNotRange trueCond ConditionalExprE cond bin_eval.simps(11) evalDet p
+          falseCond unfold_binary val_to_bool.simps(1))
+    then have falseEval: "(notCond = IntVal 32 0) \<Longrightarrow>
+                         [m,p] \<turnstile> exp[BinaryExpr BinIntegerEquals (c ? x : y) (y)]
+                               \<mapsto> intval_equals xv yv"
+      using p by (metis ConditionalExprE bin_eval.simps(11) evalDet falseCond unfold_binary)
+    have eqEvalFalse: "intval_equals yv xv = (IntVal 32 0)"
+      unfolding xvv yvv apply auto by (metis (mono_tags) bool_to_val.simps(2) yxDiff yvv xvv)
+    have trueEvalEquiv: "[m,p] \<turnstile> exp[BinaryExpr BinIntegerEquals (c ? x : y) (y)] \<mapsto> notCond"
+      by (smt (verit, best) ConditionalExpr cRange cond condNotUndef evalDet p(7) trueCond falseEval
+          trueEvalCond val_to_bool.simps(1) xv yvv intval_self_is_true intval_commute eqEvalFalse
+          evaltree_not_undef Value.distinct(1) cNotRange)
+    show ?thesis
+      using ConditionalExprE
+      by (metis cNotRange falseEval notCond trueEvalEquiv trueCond falseCond intval_self_is_true
+          yvv p(9,11) evalDet)
+  qed
+  done
+
 optimization ConditionalEqualIsRHS: "((x eq y) ? x : y) \<longmapsto> y"
   apply auto
   by (smt (verit) Value.inject(1) bool_to_val.simps(2) bool_to_val_bin.simps evalDet 
